concurrency/verif_bst_conc_nblocking.v
@@ -34,19 +34,19 @@ Hint Resolve node_data_saturate_local: saturate_local.
 
 
  Definition insert_inv (b: val) (sh: share) (x: Z) (v: val) ( g_root:gname) gv (g:gname)  (inv_names : invG) (P:mpred) (AS:mpred) (ref:val): environ -> mpred :=
-( EX np: val, EX g_current:gname, EX nodeinfos: list(gname*node_info), EX n1:number, EX n2:number,
+( EX np: val, EX g_current:gname,EX n1:number, EX n2:number,
 PROP (check_key_exist' x (n1,n2) = true)
 LOCAL (temp _ref ref; temp _temp np; temp _t b; temp _x (vint x); temp _value v; gvars gv)
 SEP ( |>P; AS && cored;in_tree g_current (n1,n2) np g; mem_mgr gv; malloc_token Ews (tptr Tvoid) ref * data_at Ews (tptr Tvoid) (vint 0) ref; 
-   nodebox_rep sh b g_root g ; iter_sepcon (fun info => ghost_snap  (snd info) (fst info)) nodeinfos
+   nodebox_rep sh b g_root g 
    ))%assert.
    
    
 Definition node_data_without_value (info: option ghost_info) g  tp lp rp  (range:number * number)  :=  
-(match info with Some data =>  EX sh, !!(readable_share sh) &&  data_at sh t_struct_tree (Vint (Int.repr data.1.1.1),(data.1.1.2,(lp,rp))) tp * in_tree  data.1.2 ( fst range, Finite_Integer (data.1.1.1)) lp g * in_tree data.2 ( Finite_Integer (data.1.1.1), snd range) rp g | None => !!(tp = nullval /\ lp = nullval /\ rp = nullval) && emp end).
+(match info with Some data =>  EX sh, !!(readable_share sh /\ Int.min_signed <= data.1.1.1 <= Int.max_signed/\ is_pointer_or_null lp /\ is_pointer_or_null rp /\ is_pointer_or_null data.1.1.2) &&  data_at sh t_struct_tree (Vint (Int.repr data.1.1.1),(data.1.1.2,(lp,rp))) tp * in_tree  data.1.2 ( fst range, Finite_Integer (data.1.1.1)) lp g * in_tree data.2 ( Finite_Integer (data.1.1.1), snd range) rp g | None => !!(tp = nullval /\ lp = nullval /\ rp = nullval) && emp end).
 
 Lemma node_data_without_value_R: forall (info: option ghost_info) g  tp lp rp  (range:number *number),  node_data_without_value info g tp  lp rp  range |-- if (eq_dec tp nullval) then !!(info = None /\ lp = nullval /\ rp = nullval) && emp  else 
-EX data, EX sh, !!(readable_share sh/\ info = Some data) &&   data_at sh t_struct_tree (Vint (Int.repr data.1.1.1),(data.1.1.2,(lp,rp))) tp * in_tree data.1.2( fst range, Finite_Integer data.1.1.1) lp g * in_tree data.2 ( Finite_Integer data.1.1.1, snd range) rp g.
+EX data, EX sh, !!(readable_share sh/\ info = Some data  /\ Int.min_signed <= data.1.1.1 <= Int.max_signed/\ is_pointer_or_null lp /\ is_pointer_or_null rp /\  is_pointer_or_null data.1.1.2) &&   data_at sh t_struct_tree (Vint (Int.repr data.1.1.1),(data.1.1.2,(lp,rp))) tp * in_tree data.1.2( fst range, Finite_Integer data.1.1.1) lp g * in_tree data.2 ( Finite_Integer data.1.1.1, snd range) rp g.
 Proof.
 intros. unfold node_data_without_value.
 destruct info.
@@ -83,24 +83,27 @@ Intros ref.
 forward.
  eapply semax_pre; [
     | apply (semax_loop _ (insert_inv b sh x v g_root gv g inv_names P AS ref) (insert_inv b sh x v g_root gv g inv_names P AS ref) )]. 
-{ intros. unfold insert_inv.  Exists b g_root (@nil (gname *node_info)).  unfold nodebox_rep in *. Intros tp lp. Exists Neg_Infinity Pos_Infinity tp lp. sep_apply (in_tree_split g_root ( Neg_Infinity, Pos_Infinity) b g) . entailer!. unfold check_key_exist'. simpl. cancel. 
-}
-* unfold insert_inv. Intros np g_current nodeinfos n1 n2.
+
+* (* Precondition *) 
+   intros. unfold insert_inv.  Exists b g_root.  unfold nodebox_rep in *. Intros tp lp. Exists Neg_Infinity Pos_Infinity tp lp. sep_apply (in_tree_split g_root ( Neg_Infinity, Pos_Infinity) b g) . entailer!.
+
+*  (* Loop body *)
+   unfold insert_inv. Intros np g_current n1 n2. 
    forward. 
    sep_apply cored_dup.
    sep_apply in_tree_split. 
    Intros.
+   (* tp = atomic_load_ptr(temp) *)
    forward_call (np, top, empty, fun tp : val => |> P * EX n n0:number, EX lp:val, EX rp:val, EX info: option ghost_info, !! (check_key_exist' x (n, n0) = true) && ghost_snap (n, n0,info) g_current * node_data_without_value info g tp lp rp  (n,n0) , inv_names).
-    { subst Frame;instantiate (1 := [AS && cored; in_tree g_current (n1, n2) np g; mem_mgr gv; malloc_token Ews (tptr Tvoid) ref;  data_at Ews (tptr Tvoid) (vint 0) ref ; nodebox_rep sh b g_root g; iter_sepcon (λ info : own.gname * (number * number * option ghost_info), ghost_snap info.2 info.1)
-      nodeinfos]).  simpl;cancel.
-     iIntros "(( in & [AS1 _]) & P)". 
+    { subst Frame;instantiate (1 := [AS && cored; in_tree g_current (n1, n2) np g; mem_mgr gv; malloc_token Ews (tptr Tvoid) ref;  data_at Ews (tptr Tvoid) (vint 0) ref ; nodebox_rep sh b g_root g]).  simpl;cancel.
+      iIntros "(( in & [AS1 _]) & P)". 
       iMod ("AS1" with "P") as (BST) "[Tree Tclose]". 
       iDestruct "Tree" as "(% & Tree)".
       unfold tree_rep2 at 1.
       iDestruct "Tree" as (tg) "((% & Tree) & gref)".
       iPoseProof (node_exist_in_tree with "[gref in]") as "%". iFrame. destruct H4 as [r H4]. destruct r as [n n0]. destruct H4.
       iPoseProof ( extract_node_info_from_ghost_tree_rep_2 with "Tree") as "Hadd". apply H4. intros. simpl;auto. apply (sortedness_preserved__in_ghosttree BST tg);auto.
-      iDestruct "Hadd" as ( tp o lp rp v0) "(info & Tree)".
+      iDestruct "Hadd" as ( tp o lp rp v0) "(info & Tree)". 
       unfold node_information at 1.
       iDestruct "info" as "(% & ((p & master) & info))". 
        iModIntro; iExists Ews, tp; iFrame "p".
@@ -111,13 +114,13 @@ forward.
         iMod ("master") as "[snap master]".  
         iDestruct "in" as (sh2) "in".
        iMod (own_dealloc with "in") as "_".
-       unfold node_data, node_data_without_value.
+       unfold node_data, node_data_without_value. 
        destruct o.
-        * destruct g0 as [[[k v3] g1 ] g2].  iDestruct "info" as (sh1) "((((% & v) & tp) & g1) & g2)". simpl in *.
-          apply split_readable_share in H7. destruct H7 as (sh3 & sh4 & H7 & H8 & H9). rewrite <- (data_at_share_join sh3 sh4 sh1 _ _ _). iDestruct "tp" as "(tp1 & tp2)".
+        * destruct g0 as [[[k v3] g1 ] g2].  instantiate (2 := x). instantiate (1 := v).  iDestruct "info" as (sh1) "(((((% & v) & malloc ) & tp) & g1) & g2)". simpl in *.
+         destruct H7. apply split_readable_share in H7. destruct H7 as (sh3 & sh4 & H7 & H9 & H10). rewrite <- (data_at_share_join sh3 sh4 sh1 _ _ _). iDestruct "tp" as "(tp1 & tp2)".
           rewrite (in_tree_split g1 ( n, Finite_Integer k) lp g). rewrite ( in_tree_split g2 ( Finite_Integer k, n0) rp g ). iDestruct "g1" as "(g11 & g12)". iDestruct "g2" as "(g21 & g22)".
         rewrite -> exp_sepcon2.  iExists n.  rewrite -> exp_sepcon2.  iExists n0.  rewrite -> exp_sepcon2.  iExists lp. rewrite -> exp_sepcon2. iExists rp. rewrite -> exp_sepcon2. iExists (Some (k,v3,g1,g2)). simpl. 
-        rewrite (prop_true_andp _ (ghost_snap (n, n0, (Some (k,v3,g1,g2))) g_current) ). rewrite <- !sepcon_assoc.   rewrite -> exp_sepcon2. iExists sh3. rewrite (prop_true_andp ( readable_share sh3 ) _ ).
+        rewrite (prop_true_andp _ (ghost_snap (n, n0, (Some (k,v3,g1,g2))) g_current) ). rewrite <- !sepcon_assoc.   rewrite -> exp_sepcon2. iExists sh3. rewrite (prop_true_andp ( readable_share sh3 ∧ (Int.min_signed ≤ k ∧ k ≤ Int.max_signed)∧ is_pointer_or_null lp ∧ is_pointer_or_null rp /\  is_pointer_or_null v3  ) _ ).
         iFrame .
        iApply "Tclose". 
        iFrame.
@@ -127,8 +130,8 @@ forward.
        iFrame;iSplit;auto.
        iApply "Tree".
        unfold node_information, node_data. rewrite -> exp_sepcon2.  iExists sh4.
-       iFrame. iSplit. iPureIntro;auto. auto. auto.
-       unfold range_inclusion, check_key_exist' in *.  apply andb_prop in H1. apply andb_prop in H5. destruct H1, H5. apply andb_true_intro. split. apply less_than_equal_less_than_transitivity with (b := n1). apply H5. apply H1. assert (less_than (Finite_Integer x) n0 = true). { apply less_than_less_than_equal_transitivity with (b := n2). apply H10. apply H11. } apply H12. auto.
+       iFrame. iSplit. iPureIntro;auto. auto. auto. 
+       unfold range_inclusion, check_key_exist' in *.  apply andb_prop in H1. apply andb_prop in H5. destruct H1, H5. apply andb_true_intro. split. apply less_than_equal_less_than_transitivity with (b := n1). apply H5. apply H1. assert (less_than (Finite_Integer x) n0 = true). { apply less_than_less_than_equal_transitivity with (b := n2). apply H11. apply H12. } apply H13. auto.
       *  rewrite -> exp_sepcon2.  iExists n.  rewrite -> exp_sepcon2.  iExists n0.  rewrite -> exp_sepcon2.  iExists lp. rewrite -> exp_sepcon2. iExists rp. rewrite -> exp_sepcon2. iExists None.   rewrite (prop_true_andp _ (ghost_snap (n, n0, None) g_current) ). iDestruct "info" as "(% & info)".  rewrite (prop_true_andp _ emp). iFrame. 
           iApply "Tclose". 
           iFrame.
@@ -139,15 +142,16 @@ forward.
          iApply "Tree".
          unfold node_information, node_data. iFrame. iPureIntro. split. apply H7. auto. apply H7.
          unfold range_inclusion, check_key_exist' in *.  apply andb_prop in H1. apply andb_prop in H5. destruct H1, H5. apply andb_true_intro. split. apply less_than_equal_less_than_transitivity with (b := n1). apply H5. apply H1. assert (less_than (Finite_Integer x) n0 = true). { apply less_than_less_than_equal_transitivity with (b := n2). apply H7. apply H8. } apply H9.
-  }
+  } 
  Intro tp.
  Intros n n0 lp rp info. 
  forward_if.
- - intros. 
+ - (* then clause *)
+  intros. 
   forward_call (t_struct_tree, gv).
   { split; simpl; [ rep_omega | auto ]. }
   Intros p.
-  forward.
+  forward. (*p->key = x;*)
  forward_call(v).
  Intro v1.
  forward.
@@ -158,16 +162,16 @@ forward.
  Intro rp1.
  forward.
  sep_apply node_data_without_value_R. subst. simpl. Intros.
- sep_apply cored_dup.
  pose proof split_Ews as share.
  destruct share as [ sh1 share]. destruct share as [ sh2 share]. destruct share. destruct H7.
  rewrite <- ( data_at_share_join sh1 sh2 Ews _ _ _ H8).
+ focus_SEP 9.
+ sep_apply cored_dup.
+ (* atomic_CAS_ptr(temp, ref, p) *)
  forward_call (np, Ews, ref, (vint 0), p, top, empty,
-        fun vp : val =>   (if eq_dec vp (vint 0) then  Q else ( |> P * EX o1: node_info, ghost_snap o1 g_current * bst_conc_nblocking_spec.atomic_ptr_at Ews (vint 0) rp1 * bst_conc_nblocking_spec.atomic_ptr_at Ews (vint 0) lp1 * bst_conc_nblocking_spec.atomic_ptr_at Ews v v1 * malloc_token Ews t_struct_tree p * data_at sh1 t_struct_tree (vint x, (v1, (lp1, rp1))) p ))  *
-          (iter_sepcon (λ info : own.gname * node_info,
-        ghost_snap info.2 info.1) nodeinfos), inv_names).
-        {  subst Frame; instantiate (1 := [AS && cored; mem_mgr gv; malloc_token Ews (tptr Tvoid) ref; data_at sh2 t_struct_tree (vint x, (v1, (lp1, rp1))) p; nodebox_rep sh b g_root g]). unfold fold_right_sepcon. cancel.
-         iIntros "((((((((([AS1 _] & rp1) & lp1) & v1 ) & token ) & p ) &P) &snap) & in)&snaps)".
+        fun vp : val =>   (if eq_dec vp (vint 0) then  Q else ( |> P *  in_tree g_current (n1, n2) np g * bst_conc_nblocking_spec.atomic_ptr_at Ews (vint 0) rp1 * bst_conc_nblocking_spec.atomic_ptr_at Ews (vint 0) lp1 * bst_conc_nblocking_spec.atomic_ptr_at Ews v v1 * malloc_token Ews t_struct_tree p * data_at sh1 t_struct_tree (vint x, (v1, (lp1, rp1))) p )), inv_names).
+        {  subst Frame; instantiate (1 := [ mem_mgr gv; AS && cored; malloc_token Ews (tptr Tvoid) ref; data_at sh2 t_struct_tree (vint x, (v1, (lp1, rp1))) p; nodebox_rep sh b g_root g]). unfold fold_right_sepcon. cancel.
+         iIntros "(((((((([AS1 _] & rp1) & lp1) & v1 ) & token ) & p ) &P) &snap) & in)".
          iMod ("AS1" with "P") as (BST) "[Tree Tclose]". 
          iDestruct "Tree" as "(% & Tree)".
          unfold tree_rep2 at 1.
@@ -184,10 +188,10 @@ forward.
         iIntros "np".
        iDestruct "Tclose" as "[_ Tclose ]".
        iMod (ghost_node_alloc with "[$]") as (gl) "lg". apply find_ghost_set_finite.
-       iDestruct "lg" as "(((lg & ref) & in) & inl)".
+       iDestruct "lg" as "((((% & lg) & ref) & in) & inl)".
        instantiate(1 :=  lp1). instantiate(1 := (n3, Finite_Integer x)). instantiate (1 := None). 
        iMod (ghost_node_alloc with "[ref in]") as (gr) "rg". instantiate (1 := (map_upd (find_ghost_set tg g_root (Neg_Infinity, Pos_Infinity) b) gl (n3, Finite_Integer x, lp1))). apply finite_upd. apply find_ghost_set_finite. iFrame.
-       iDestruct "rg" as "(((rg & ref) & in) & inr)".
+       iDestruct "rg" as "((((% & rg) & ref) & in) & inr)".
         iDestruct "in" as (sh5) "in".
        iMod (own_dealloc with "in") as "_".
        instantiate(1 := rp1).  instantiate(1 := (Finite_Integer x, n4)). instantiate (1 := None).
@@ -196,8 +200,8 @@ forward.
        instantiate (1 := v).  instantiate (1 := x). 
        iSpecialize ("Tree" $! gl gr p).
         iPoseProof (node_data_R with "info") as "info". 
-       subst tp. iSimpl in "info". iDestruct "info" as "[% _]". 
-       destruct H14. subst o1.       
+       subst tp. iSimpl in "info". iDestruct "info" as "[% _]".  
+       destruct H16. subst o1.       
        iMod (snap_master_update1(ORD := range_order) _ _ _ (n3,n4,Some (x, v1, gl, gr))  with "[$snap $master]") as "[snap master]".
        { simpl. split. rewrite andb_true_intro. auto. split;apply less_than_equal_itself. auto. }
        iMod (own_dealloc with "snap") as "_".
@@ -208,22 +212,22 @@ forward.
        unfold node_information,node_data.
        assert (check_key_exist' x (n3, n4) = true). { unfold range_inclusion, check_key_exist' in *. apply andb_prop in H12. apply andb_prop in H1. destruct H1, H12. 
        rewrite andb_true_intro. auto.  split;auto.  apply less_than_equal_less_than_transitivity with  (b := n1). apply H12. apply H1.
-       apply less_than_less_than_equal_transitivity with  (b := n2). apply H14. apply H16. }     
-       iSpecialize ("Tree" with "[rp1 lp1 v1 p np lg inl rg inr master ]") . instantiate(1:= rp1).  instantiate(1:= lp1).   instantiate(1:= v1). 
-       rewrite prop_true_andp. rewrite -> exp_sepcon2.  repeat rewrite exp_sepcon1.  iExists sh1. iFrame. iPureIntro. split;auto. destruct H15. repeat split;auto. admit.
+       apply less_than_less_than_equal_transitivity with  (b := n2). apply H16. apply H18. }     
+       iSpecialize ("Tree" with "[rp1 lp1 v1 p token np lg inl rg inr master ]") . instantiate(1:= rp1).  instantiate(1:= lp1).   instantiate(1:= v1). 
+       rewrite prop_true_andp. rewrite -> exp_sepcon2.  repeat rewrite exp_sepcon1.  iExists sh1. iFrame. iPureIntro. split;auto. destruct H17. repeat split;auto. destruct H. auto. destruct H;auto. 
+       destruct H17. repeat split;auto.
         iDestruct "Tree" as "(% & Tree)".
-        rewrite prop_true_andp. apply (key_not_exist_in_tree _ _ _ x) in H16.
-       rewrite (update_ghost_tree_with_insert x v v1 tg gl gr g_root _ lp1 rp1 g_current n3 n4 np b). iFrame. admit.
-       auto. auto. intros. simpl;auto. apply (sortedness_preserved__in_ghosttree BST _ H10 H9). simpl;auto. apply insert_preserved_in_ghost_tree. auto. auto.
+        rewrite prop_true_andp.  assert (H19 := H18). apply (key_not_exist_in_tree _ _ _ x) in H18.
+       rewrite (update_ghost_tree_with_insert x v v1 tg gl gr g_root _ lp1 rp1 b n3 n4 None). iFrame. auto. apply H14. apply H15. apply H18.
+        apply (sortedness_preserved__in_ghosttree BST _ H10 H9). intros. simpl;auto. simpl;auto.  intros. simpl;auto.  apply (sortedness_preserved__in_ghosttree BST _ H10 H9). auto. apply insert_preserved_in_ghost_tree. auto. auto.
        
-       }
+       } 
        iIntros "np".
        iMod (snap_master_update1(ORD := range_order) _ _ _ (n3, n4, o1) with "[$snap $master]") as "[snap master]".
        {  split. apply range_iteself. simpl. destruct o1;auto. }
-        iDestruct "Tclose" as "[Tclose _]".
-         iDestruct "in" as (sh5) "in".
-       iMod (own_dealloc with "in") as "_". 
-        rewrite -> exp_sepcon2.  rewrite exp_sepcon1. iExists (n3,n4,o1). iFrame.
+        iMod (own_dealloc with "snap") as "_".
+        iDestruct "Tclose" as "[Tclose _]".  iFrame.
+
         iApply "Tclose".  rewrite prop_true_andp.
        unfold tree_rep2.
        iExists tg.
@@ -233,16 +237,108 @@ forward.
        iFrame. auto.
      }       
      Intro result.
-     focus_SEP 2.     
-      match goal with |- semax _ (PROP () (LOCALx (_ :: _ :: ?Q) (SEPx (_ :: ?R)))) _ _ =>
-        forward_if (PROP () ((LOCALx Q) (SEPx (  |> P * (EX o1 : node_info,
-      ghost_snap o1 g_current * bst_conc_nblocking_spec.atomic_ptr_at Ews (vint 0) rp1 *
-      bst_conc_nblocking_spec.atomic_ptr_at Ews (vint 0) lp1 *
-      bst_conc_nblocking_spec.atomic_ptr_at Ews v v1 * malloc_token Ews t_struct_tree p *
-      data_at sh1 t_struct_tree (vint x, (v1, (lp1, rp1))) p) :: R)))) end.
-      --  if_tac; [discriminate|]. Intros o1.
-           forward_call (atomic_ptr, v1, gv). 
-  
+     focus_SEP 1.
+     forward_if. (* if (!result) *)
+      --  if_tac; [discriminate|]. Intros. 
+           forward_call (v1). Exists v. entailer!.
+           forward_call (lp1). Exists (vint 0). entailer!.
+           forward_call (rp1). Exists (vint 0). entailer!. 
+           focus_SEP 8. focus_SEP 4.
+           assert_PROP (p <> nullval). { entailer!. } 
+           forward_call(t_struct_tree, p, gv ).
+           {  if_tac.
+             - contradiction.
+             - erewrite data_at_share_join. entailer!. auto.
+           }
+           forward.
+           Exists np g_current n1 n2.
+           entailer!.
+   --   if_tac; [|contradiction]. Intros.
+          assert_PROP (ref <> nullval). { entailer!. } 
+          forward_call((tptr Tvoid), ref, gv).
+          { if_tac.
+            - contradiction.
+            - entailer!. 
+          }
+    forward. unfold nodebox_rep. Intros tp lp. rewrite <- !sepcon_assoc. Exists tp (p :: lp). simpl. rewrite <- !sepcon_assoc. Exists sh2. entailer!. admit. (* extra AS && cored, need to fix*)
+ -  (* else clause *)
+    Intros.  
+    sep_apply node_data_without_value_R. 
+    if_tac; [contradiction|]. Intros data sh1.
+    forward.
+    destruct data as [[[ k vp] g1] g2]. simpl. simpl in H7.
+    forward_if; [ | forward_if ].
+    --  (* Inner if, then clause: x<y *)   
+         gather_SEP ( in_tree g2 (Finite_Integer k, n0) rp g) (ghost_snap (n, n0, info) g_current) (in_tree g_current (n1, n2) np g).
+         viewshift_SEP 0 (emp). 
+         { go_lower. unfold in_tree, ghost_snap, ghost_part. Intros sh4 sh5.  iIntros "[[H1 H2] H3]".
+           iMod (own_dealloc with "H1"); iMod (own_dealloc with "H2"); iMod (own_dealloc with "H3"); eauto.
+         }
+         forward. unfold nodebox_rep. Intros tp0 lp0.
+         Exists lp g1 n (Finite_Integer k). Exists tp0 (tp :: lp0). simpl iter_sepcon. Exists sh1. 
+          entailer!.
+         { unfold check_key_exist' in *. apply andb_true_intro. split. apply andb_prop in H2. destruct H2. auto. simpl.  rewrite Z.ltb_lt. omega. } 
+    -- (* Inner if, second branch:  y<x *)
+         gather_SEP ( in_tree g1 (n, Finite_Integer k) lp g) (ghost_snap (n, n0, info) g_current) (in_tree g_current (n1, n2) np g).
+         viewshift_SEP 0 (emp). 
+         { go_lower. unfold in_tree, ghost_snap, ghost_part. Intros sh4 sh5.  iIntros "[[H1 H2] H3]".
+           iMod (own_dealloc with "H1"); iMod (own_dealloc with "H2"); iMod (own_dealloc with "H3"); eauto.
+         }
+         forward. unfold nodebox_rep. Intros tp0 lp0.
+         Exists rp g2  (Finite_Integer k) n0. Exists tp0 (tp :: lp0). simpl iter_sepcon. Exists sh1. entailer!.
+         { unfold check_key_exist' in *. apply andb_true_intro. split.  simpl.  rewrite Z.ltb_lt. omega.  apply andb_prop in H2. destruct H2. auto. } 
+         
+    --  (* x = y *)
+         forward. 
+         focus_SEP 5. 
+         forward_call ( vp, v, top, empty, Q , inv_names).
+         {  subst Frame. instantiate (1 := [ mem_mgr gv; malloc_token Ews (tptr Tvoid) ref; data_at Ews (tptr Tvoid) (vint 0) ref; data_at sh1 t_struct_tree (vint k, (vp, (lp, rp))) tp; nodebox_rep sh b g_root g]).  unfold fold_right_sepcon. cancel.
+         iIntros "((((([AS1 _] & in1) & in2 ) & P ) & snap) & in)".
+          iMod ("AS1" with "P") as (BST) "[Tree Tclose]". 
+         iDestruct "Tree" as "(% & Tree)".
+         unfold tree_rep2 at 1.
+         iDestruct "Tree" as (tg) "((% & Tree) & gref)".
+         iPoseProof (node_exist_in_tree with "[gref in]") as "%". iFrame. destruct H13 as [r H13]. destruct r as [n3 n4]. destruct H13.
+         iPoseProof ( extract_node_info_from_ghost_tree_rep_2 with "Tree") as "Hadd". eauto. intros. simpl;auto. apply (sortedness_preserved__in_ghosttree BST tg );auto.
+        iDestruct "Hadd" as (tp0 o lp0 rp0 v0) "(info & Tree)". instantiate (1 := v). instantiate (1 := x).
+        unfold node_information at 1.
+       iDestruct "info" as "(% & ((ap & master) & info))". 
+       iCombine "snap master" as "master"; rewrite -> snap_master_join1. 
+       iDestruct "master" as "[ % master]".
+       destruct H16.  rewrite H6 in H17. simpl in H17.  rewrite <- H17. unfold node_data.
+       iDestruct "info" as (sh4) "(((((% & vp) & token ) & tp ) & in11 ) & in21)".
+       unfold in_tree, ghost_part at 1. unfold in_tree, ghost_part at 1. unfold in_tree, ghost_part at 1.
+       iDestruct "in1" as (sh8) "in1". iMod (own_dealloc with "in1") as "_".
+        iDestruct "in2" as (sh9) "in2". iMod (own_dealloc with "in2") as "_".
+       iDestruct "in" as (sh10) "in". iMod (own_dealloc with "in") as "_".
+       iModIntro. iExists Ews. rewrite (bst.bst_conc_nblocking_spec.atomic_ptr_at__ Ews v0 _). iFrame "vp".
+       iSplitL ""; [iSplit; auto; iPureIntro; split; auto; tauto|].
+        iIntros "np".
+       iDestruct "Tclose" as "[_ Tclose ]".
+        iApply ("Tclose"  $! tt). simpl.
+       iSplitL. iSplit. iPureIntro. apply insert_sorted. auto.
+       unfold tree_rep2. iExists  (insert_ghost x v vp tg g1 lp0 g2 rp0).
+       assert ( x = k). { omega. }
+       assert (check_key_exist' x (n3, n4) = true). { unfold range_inclusion, check_key_exist' in *. apply andb_prop in H14. apply andb_prop in H1. destruct H1, H14. 
+       rewrite andb_true_intro. auto.  split;auto.  apply less_than_equal_less_than_transitivity with  (b := n1). apply H14. apply H1.
+       apply less_than_less_than_equal_transitivity with  (b := n2). apply H20. apply H21. }     
+       iSpecialize ("Tree" with "[np ap tp token  in11  in21 master ]") . instantiate (1 := g2). instantiate (1:=g1). instantiate (1 := vp). 
+       rewrite prop_true_andp. unfold node_information,node_data. rewrite -> exp_sepcon2.  repeat rewrite exp_sepcon1.  iExists sh4. simpl.  destruct H19.  iFrame.  iPureIntro. split;auto.
+       destruct H19. split;auto.
+       iDestruct "Tree" as "(% & Tree)".
+       rewrite (update_ghost_tree_with_insert2 x v vp tg g1 g2 g_root (Neg_Infinity, Pos_Infinity) lp0 rp0 b). iFrame. iPureIntro. split;auto. 
+       apply insert_preserved_in_ghost_tree;auto. split;auto. apply (sortedness_preserved__in_ghosttree BST tg H12 H11). auto.
+   }
+   assert_PROP (ref <> nullval). { entailer!. } 
+   forward_call((tptr Tvoid), ref, gv).
+      { if_tac.
+            - contradiction.
+            - entailer!. 
+      }
+  forward. unfold nodebox_rep. Intros tp0 lp0. rewrite <- !sepcon_assoc. Exists tp0 (tp :: lp0). simpl. rewrite <- !sepcon_assoc. Exists sh1. entailer!.
+* (* After the loop *)
+   forward. normalize. 
+    
 Admitted.
 
 
